ironfleet/ravana/DistributedSystem.i.dfy
@@ -17,17 +17,17 @@ module DistributedSystem_i {
     && SeqIsUnique([config.node_logger] + config.node_controllers + config.node_switches)
 
     && |config.node_controllers| > 0
-    && (forall e :: e in rs.server_controllers <==> e in config.node_controllers)
+    && (forall e :: e in rs.controllers <==> e in config.node_controllers)
     && (forall index :: 0 <= index < |config.node_controllers| ==>
-            NodeInit_Controller(rs.server_controllers[config.node_controllers[index]],
+            NodeInit_Controller(rs.controllers[config.node_controllers[index]],
                                 index,
                                 config)
        )
 
     && |config.node_switches| > 0
-    && (forall e :: e in rs.server_switches <==> e in config.node_switches)
+    && (forall e :: e in rs.switches <==> e in config.node_switches)
     && (forall index :: 0 <= index < |config.node_switches| ==>
-            NodeInit_Switch(rs.server_switches[config.node_switches[index]],
+            NodeInit_Switch(rs.switches[config.node_switches[index]],
                            index,
                            config)
        )
@@ -43,27 +43,27 @@ module DistributedSystem_i {
         (if rs.environment.nextStep.actor == rs.endpoint_logger then
             RS_NextOneServer_Logger(rs, rs',
                 rs.environment.nextStep.actor, rs.environment.nextStep.ios) &&
-            rs.server_controllers == rs'.server_controllers &&
-            rs.server_switches == rs'.server_switches
-        else if rs.environment.nextStep.actor in rs.server_controllers then
+            rs.controllers == rs'.controllers &&
+            rs.switches == rs'.switches
+        else if rs.environment.nextStep.actor in rs.controllers then
             RS_NextOneServer_Controller(rs, rs',
                 rs.environment.nextStep.actor, rs.environment.nextStep.ios) &&
             rs.server_logger == rs'.server_logger &&
-            rs.server_switches == rs'.server_switches
-        else if rs.environment.nextStep.actor in rs.server_switches then
+            rs.switches == rs'.switches
+        else if rs.environment.nextStep.actor in rs.switches then
             RS_NextOneServer_Switch(rs, rs',
                 rs.environment.nextStep.actor, rs.environment.nextStep.ios) &&
             rs.server_logger == rs'.server_logger &&
-            rs.server_controllers == rs'.server_controllers
+            rs.controllers == rs'.controllers
         else
             rs.server_logger == rs'.server_logger &&
-            rs.server_controllers == rs'.server_controllers &&
-            rs.server_switches == rs'.server_switches
+            rs.controllers == rs'.controllers &&
+            rs.switches == rs'.switches
         )
       else
         rs.server_logger == rs'.server_logger &&
-        rs.server_controllers == rs'.server_controllers &&
-        rs.server_switches == rs'.server_switches
+        rs.controllers == rs'.controllers &&
+        rs.switches == rs'.switches
     )
   }
 
@@ -75,19 +75,19 @@ module DistributedSystem_i {
   }
 
   predicate RS_NextOneServer_Controller(rs: RState, rs': RState, id: EndPoint, ios: seq<RavanaIo>)
-  requires id in rs.server_controllers
+  requires id in rs.controllers
   {
-        id in rs'.server_controllers
-     && NodeNext_Controller(rs.server_controllers[id], rs'.server_controllers[id], ios)
-     && rs'.server_controllers == rs.server_controllers[id := rs'.server_controllers[id]]
+        id in rs'.controllers
+     && NodeNext_Controller(rs.controllers[id], rs'.controllers[id], ios)
+     && rs'.controllers == rs.controllers[id := rs'.controllers[id]]
   }
 
   predicate RS_NextOneServer_Switch(rs: RState, rs': RState, id: EndPoint, ios: seq<RavanaIo>)
-  requires id in rs.server_switches
+  requires id in rs.switches
   {
-        id in rs'.server_switches
-     && NodeNext_Switch(rs.server_switches[id], rs'.server_switches[id], ios)
-     && rs'.server_switches == rs.server_switches[id := rs'.server_switches[id]]
+        id in rs'.switches
+     && NodeNext_Switch(rs.switches[id], rs'.switches[id], ios)
+     && rs'.switches == rs.switches[id := rs'.switches[id]]
   }
 
 }
