ironfleet/ravana/RefinementProof/SwitchRecvCommandSendAck.dfy
@@ -19,17 +19,17 @@ module Refinement_Proof_SwitchRecvCommandSendAck {
     && rs.environment.nextStep.LEnvStepHostIos?
     && rs.endpoint_logger == rs'.endpoint_logger
     && rs.initControllerState == rs'.initControllerState
-    && rs.environment.nextStep.actor in rs.server_switches
-    && rs.environment.nextStep.actor in rs'.server_switches
+    && rs.environment.nextStep.actor in rs.switches
+    && rs.environment.nextStep.actor in rs'.switches
     && Node_SwitchRecvCommandSendAck(
-                rs.server_switches[rs.environment.nextStep.actor],
-                rs'.server_switches[rs.environment.nextStep.actor],
+                rs.switches[rs.environment.nextStep.actor],
+                rs'.switches[rs.environment.nextStep.actor],
                 command_id,
                 rs.environment.nextStep.ios)
-    && rs.server_controllers == rs'.server_controllers
+    && rs.controllers == rs'.controllers
     && rs.server_logger == rs'.server_logger
-    && rs'.server_switches == rs.server_switches[
-        rs.environment.nextStep.actor := rs'.server_switches[rs.environment.nextStep.actor]]
+    && rs'.switches == rs.switches[
+        rs.environment.nextStep.actor := rs'.switches[rs.environment.nextStep.actor]]
   }
 
   lemma lemma_refines_SwitchEventSend(rs: RState, rs': RState, command_id: int)
@@ -45,19 +45,19 @@ module Refinement_Proof_SwitchRecvCommandSendAck {
 
     lemma_refinement_switchStates_eq(rs, rs', command_id);
 
-    assert refinement_switchStates(rs.server_switches)
-        == refinement_switchStates(rs'.server_switches);
+    assert refinement_switchStates(rs.switches)
+        == refinement_switchStates(rs'.switches);
 
     assert refinement_controllerState(rs.server_logger.log, rs.initControllerState)
         == refinement_controllerState(rs'.server_logger.log, rs'.initControllerState);
 
     lemma_outstanding_commands_eq(rs, rs');
-    assert refinement_outstandingCommands(rs.server_logger.log, rs.initControllerState, rs.server_switches)
-        == refinement_outstandingCommands(rs'.server_logger.log, rs'.initControllerState, rs'.server_switches);
+    assert refinement_outstandingCommands(rs.server_logger.log, rs.initControllerState, rs.switches)
+        == refinement_outstandingCommands(rs'.server_logger.log, rs'.initControllerState, rs'.switches);
 
     lemma_outstanding_events_eq(rs, rs');
-    assert refinement_outstandingEvents(rs.server_switches, rs.server_logger.log)
-        == refinement_outstandingEvents(rs'.server_switches, rs'.server_logger.log);
+    assert refinement_outstandingEvents(rs.switches, rs.server_logger.log)
+        == refinement_outstandingEvents(rs'.switches, rs'.server_logger.log);
   }
 
   lemma lemma_packets_are_valid(rs: RState, rs': RState, command_id: int)
@@ -113,7 +113,7 @@ module Refinement_Proof_SwitchRecvCommandSendAck {
 
   lemma lemma_log_is_valid(rs: RState, rs': RState, command_id: int)
   requires conditions(rs, rs', command_id)
-  ensures log_is_valid(rs'.server_switches, rs'.server_logger.log)
+  ensures log_is_valid(rs'.switches, rs'.server_logger.log)
   {
     reveal_log_is_valid();
   }
@@ -121,22 +121,22 @@ module Refinement_Proof_SwitchRecvCommandSendAck {
   lemma lemma_accepted_commands_are_valid(rs: RState, rs': RState, command_id: int)
   requires conditions(rs, rs', command_id)
   ensures accepted_commands_are_valid(rs'.initControllerState,
-        rs'.server_switches, rs'.server_logger.log)
+        rs'.switches, rs'.server_logger.log)
   {
     reveal_accepted_commands_are_valid();
   }
 
   lemma lemma_switches_valid(rs: RState, rs': RState, command_id: int)
   requires conditions(rs, rs', command_id)
-  ensures switches_valid(rs'.server_switches)
+  ensures switches_valid(rs'.switches)
   {
     reveal_switches_valid();
   }
 
   lemma lemma_refinement_switchStates_eq(rs: RState, rs': RState, command_id: int)
   requires conditions(rs, rs', command_id)
-  ensures refinement_switchStates(rs.server_switches)
-       == refinement_switchStates(rs'.server_switches);
+  ensures refinement_switchStates(rs.switches)
+       == refinement_switchStates(rs'.switches);
   {
   }
 }
